Migrate to new defs

src/ThreadTrace.v
@@ -180,7 +180,7 @@ Definition trace_coherent traces G : Prop :=
     ⟪ IN_TRACES : traces thr tr ⟫ /\
     ⟪ PREFIX : trace_prefix (thread_trace G thr) tr ⟫.
 
-Definition trace_prefix G G' : Prop :=
+Definition exec_trace_prefix G G' : Prop :=
   forall thr, trace_prefix (thread_actid_trace G' thr) (thread_actid_trace G thr).
 
 Definition contigious_actids G : Prop := forall t, exists N,
@@ -189,7 +189,7 @@ Definition contigious_actids G : Prop := forall t, exists N,
 (* TODO: make G' prefix G *)
 Lemma trace_coherent_sub traces G G' sc sc'
     (TRACE_COH : trace_coherent traces G)
-    (PREFIX : trace_prefix G G')
+    (PREFIX : exec_trace_prefix G G')
     (SUB : sub_execution G G' sc sc') :
   trace_coherent traces G'.
 Proof using.
@@ -198,7 +198,7 @@ Admitted.
 
 Lemma trace_form_sub G G'
     (CONT : contigious_actids G)
-    (PREFIX : trace_prefix G G') :
+    (PREFIX : exec_trace_prefix G G') :
   contigious_actids G'.
 Proof using.
   admit.
